chore: split ReflectVerif into multiple files [1/?] (#1439)
The infrastructure built in ReflectVerif should live in multiple files,
with `ReflectVerif` containing only the K-induction proof. In the
subsequent PRs, we cleanup the naming convention.

SSA/Projects/InstCombine/scripts/extract-goals.py
@@ -1,0 +1,169 @@
+#!/usr/bin/env python3
+# This script extracts goal states from Lean files in the
+# 'SSA/Projects/InstCombine/tests/proofs' directory.
+# This ensures that there is one goal state per file,
+# which makes scripting much easier.
+import concurrent.futures
+import subprocess
+import datetime
+import platform
+import argparse
+import shutil
+from typing import List
+from pathlib import Path
+from dataclasses import dataclass, asdict
+import pandas as pd
+import os
+import re
+import logging
+import random
+import json
+
+ROOT_DIR = subprocess.check_output(['git', 'rev-parse', '--show-toplevel']).decode('utf-8').strip()
+BENCHMARK_DIR = ROOT_DIR + '/SSA/Projects/InstCombine/tests/proofs/'
+GOALS_DIR = ROOT_DIR + '/SSA/Projects/InstCombine/tests/goals/'
+
+STATUS_FAIL = "❌"
+STATUS_GREEN_CHECK = "✅"
+STATUS_SUCCESS = "🎉"
+STATUS_PROCESSING = "🕒"
+
+def sed():
+    if platform.system() == "Darwin":
+        return "gsed"
+    return "sed"
+
+@dataclass
+class Theorem:
+    # the name of the theorem.
+    name : str
+    # the text of the theorem, including 'theorem <name> <args> := by sorry
+    text : str
+
+def extract_theorems(raw : str) -> List[Theorem]:
+    out = []
+    raw = raw.strip()
+    ss = re.findall(r'(theorem.*?:= sorry)', raw, re.DOTALL)
+    for s in ss:
+        # grab the theorem name.
+        thm_name = re.search(r'\btheorem\s+([\w._]+)', s).group(1)
+        if not thm_name:
+            logging.warning(f"{fileTitle}({file_num}): Failed to extract theorem name from theorem string {s}")
+            continue
+        thm = Theorem(name=thm_name, text=s.strip())
+        out.append(thm)
+    return out
+
+
+def run_file(db : str, file: str, file_num : int, nfiles : int, timeout : int):
+    file_path = BENCHMARK_DIR + file
+    fileTitle = file.split('.')[0]
+    EXTRACT_GOALS = "extract_goals"
+    logging.info(f"{fileTitle}: writing '{EXTRACT_GOALS}' tactic into file #{file_num}.")
+    subprocess.Popen(f'{sed()} -i -E \'s,simp_alive_benchmark,{EXTRACT_GOALS},g\' ' + file_path, cwd=ROOT_DIR, shell=True).wait()
+
+    cmd = 'lake lean ' + file_path
+    logging.info(f"{fileTitle}({file_num}/{nfiles}): running '{cmd}'")
+
+    # TODO: can check that file exists to skip.
+    p = subprocess.Popen(cmd, cwd=ROOT_DIR, stdout=subprocess.PIPE, stderr=subprocess.PIPE, shell=True, universal_newlines=True)
+    logging.info(f"{fileTitle}({file_num}/{nfiles}): running...")
+    try:
+        out, err = p.communicate(timeout=timeout)
+    except subprocess.TimeoutExpired as e:
+        logging.info(f"{file_path} - time out of {TIMEOUT} seconds reached")
+        p.kill()
+        return False
+
+    logging.info(f"{fileTitle}({file_num}/{nfiles}): done processing.")
+    if p.returncode != 0:
+        logging.error(f"{fileTitle}({file_num}/{nfiles}) {STATUS_FAIL}: Expected return code of 0, found {p.returncode}")
+
+    # split 'out' into parts that are delimited by 'theorem ... := sorry'.
+    theorems = extract_theorems(out)
+    with open(db, "a") as f:
+        f.write(json.dumps({
+            "fileTitle": fileTitle,
+            "contents": out,
+            "theorems": [asdict(t) for t in theorems]
+            }) + "\n")
+
+    for t in theorems:
+        path = Path(GOALS_DIR) / f"{fileTitle}_{t.name}.lean"
+        with open(path, 'w') as f:
+            f.write(t.text)
+            logging.info(f"{fileTitle}({file_num}/{nfiles}): {STATUS_GREEN_CHECK} Extracted {path}")
+    return True
+
+def process(db : str, jobs: int, nfiles: int, timeout : int):
+    tactic_auto_path = f'{ROOT_DIR}/SSA/Projects/InstCombine/TacticAuto.lean'
+
+    if os.path.exists(db):
+        os.remove(db)
+
+    logging.info(f"Clearing git state of '{BENCHMARK_DIR}' with 'git checkout --'")
+    gco = subprocess.Popen(f'git checkout -- {BENCHMARK_DIR}', cwd=ROOT_DIR, shell=True)
+    gco.wait()
+    assert gco.returncode == 0, f"git checkout -- {BENCHMARK_DIR} should succeed."
+
+
+    raw_files = list(os.listdir(BENCHMARK_DIR))
+
+    files = []
+    for ix, file in enumerate(raw_files):
+        if "_proof" in file:
+            files.append(file)
+            if len(files) > nfiles:
+                break # quit if we are not doing a production run after 5 files.
+
+    total = len(files)
+    logging.info(f"total #files to process: {total}")
+    num_completed = 0
+    future2file = {}
+    with concurrent.futures.ThreadPoolExecutor(max_workers=jobs) as executor:
+        for ix, file in enumerate(files):
+            future = executor.submit(run_file, db, file, ix + 1, total, timeout)
+            future2file[future] = file
+
+    total = len(future2file)
+    assert len(future2file) == len(files)
+    for future in concurrent.futures.as_completed(future2file):
+        file = future2file[future]
+        try:
+            success = future.result()
+        except Exception as exc:
+            success = False
+            logging.error('%r FAILED with exception: %s' % (file, exc))
+        else:
+            if not success:
+                logging.error('%r FAILED run' % (file))
+
+        percentage = ((ix + 1) / total) * 100
+        status_symbol = STATUS_SUCCESS if success else STATUS_FAIL
+        logging.info(f'{status_symbol} completed {file} ({percentage:.1f}%)')
+        num_completed += 1
+        logging.info(f"total #files processed: {num_completed}/{total}")
+
+    if num_completed != total:
+        logging.error(f"Expected {total} files to be processed, but got {num_completed} completed futures.")
+
+def setup_logging(db_name : str):
+    # Set up the logging configuration
+    logging.basicConfig(level=logging.DEBUG,
+        format='%(asctime)s - %(levelname)s - %(message)s',
+        handlers=[logging.FileHandler(f'{db_name}.log', mode='a'), logging.StreamHandler()])
+
+if __name__ == "__main__":
+  current_time = datetime.datetime.now().strftime('%Y-%m-%d-%H:%M:%S')
+  nproc = os.cpu_count()
+  parser = argparse.ArgumentParser(prog='extract-goals')
+  default_db = f'extract-goals-{current_time}.jsonl'
+  parser.add_argument('--db', default=default_db, help='path to jsonl database')
+  parser.add_argument('-j', '--jobs', type=int, default=1)
+  parser.add_argument('--nfiles', type=int, default=4, help="number of files to extract")
+  parser.add_argument('--timeout', type=int, default=600, help="timeout in seconds for each file processing")
+  args = parser.parse_args()
+  setup_logging(args.db)
+  logging.info(args)
+  process(args.db, jobs=args.jobs, nfiles=args.nfiles, timeout=args.timeout)
+
