SSA/Core/Tactic/ExtractGoals.lean
@@ -1,0 +1,72 @@
+/-
+Copyright (c) 2017 Simon Hudon. All rights reserved.
+Released under Apache 2.0 license as described in the file LICENSE.
+
+Authors: Simon Hudon, Kyle Miller, Damiano Testa
+
+Extracts multiple goals from a theorem.
+Adapted from Mathlib's `ExtractGoals` module.
+Adaptor: Siddharth Bhat
+-/
+import Mathlib.Init
+import Lean.Elab.Tactic.ElabTerm
+import Lean.Meta.Tactic.Cleanup
+import Lean.PrettyPrinter
+import Batteries.Lean.Meta.Inaccessible
+
+/-!
+#  `extract_goals`: Format the current goals as a stand-alone example.
+
+-/
+
+syntax (name := extractGoal) "extract_goals" : tactic
+
+open Lean Meta Elab Tactic in
+elab_rules : tactic
+  | `(tactic| extract_goals) => do
+    let name ← mkAuxDeclName `extracted
+    let msgs ← withoutModifyingEnv <| withoutModifyingState do
+      let mut ix := 1
+      let mut msgs := #[]
+      for g in ← getGoals do
+        let name := name ++ Name.mkSimple s!"_{ix}"
+        ix := ix + 1
+        let (g, _) ← g.renameInaccessibleFVars
+        let (_, g) ← g.revert (clearAuxDeclsInsteadOfRevert := true) (← g.getDecl).lctx.getFVarIds
+        let ty ← instantiateMVars (← g.getType)
+        if ty.hasExprMVar then
+          -- TODO: turn metavariables into new hypotheses?
+          throwError "Extracted goal has metavariables: {ty}"
+        let ty ← Term.levelMVarToParam ty
+        let seenLevels := collectLevelParams {} ty
+        let levels := (← Term.getLevelNames).filter
+                        fun u => seenLevels.visitedLevel.contains (.param u)
+        addAndCompile <| Declaration.axiomDecl
+          { name := name
+            levelParams := levels
+            isUnsafe := false
+            type := ty }
+        let sig ← addMessageContext <| MessageData.signature name
+        let cmd := if ← Meta.isProp ty then "theorem" else "def"
+        msgs := msgs.push <| m!"{cmd} {sig} := sorry"
+        logError "xx"
+      pure msgs
+    for msg in msgs do
+      logInfo msg
+
+
+/--
+info: theorem _example.extracted_1._1 (P Q R : Prop) : P := sorry
+---
+info: theorem _example.extracted_1._2 (P Q R : Prop) : Q := sorry
+---
+info: theorem _example.extracted_1._3 (P Q R : Prop) : R := sorry
+---
+warning: declaration uses 'sorry'
+-/
+#guard_msgs in example (P Q R : Prop) : P ∧ Q ∧ R := by
+    constructor <;> try constructor
+    extract_goals
+    all_goals sorry
+
+
